EE546_W25.lean
@@ -1,3 +1,3 @@
 -- This module serves as the root of the `EE546_W25` library.
 -- Import modules here that should be built as part of the library.
-import EE546_W25.Lectures.Lean
+import EE546_W25.Homework.ComplexInt
